Relocate split-related definitions
We will need at least some of these in the proof of recomposition as
well as in the main theorem.

security/Split.v
@@ -10,3 +10,40 @@ Proof.
 Defined.
 
 Definition split := compartment -> side.
+
+
+Require Import Csyntax Asm.
+
+(* Section Split. *)
+
+    Definition c_has_side (s: split) (lr: side) (p: Csyntax.program) :=
+      List.Forall (fun '(id, gd) =>
+                     match gd with
+                     | Gfun (Ctypes.Internal f) => s (comp_of f) = lr
+                     | _ => True
+                     end)
+        (Ctypes.prog_defs p).
+
+    Definition asm_has_side (s: split) (lr: side) (p: Asm.program) :=
+      List.Forall (fun '(id, gd) =>
+                     match gd with
+                     | Gfun (Internal f) => s (comp_of f) = lr
+                     | _ => True
+                     end)
+        (prog_defs p).
+
+    Definition c_compatible (s: split) (p p': Csyntax.program) :=
+      c_has_side s Left p /\ c_has_side s Right p'.
+
+    Definition asm_compatible (s: split) (p p': Asm.program) :=
+      asm_has_side s Left p /\ asm_has_side s Right p'.
+
+    Lemma link_compatible: forall s p p',
+        c_compatible s p p' ->
+        Ctypes.prog_pol p = Ctypes.prog_pol p' ->
+        exists W, link p p' = Some W.
+    Proof.
+      admit.
+    Admitted.
+
+(* End Split. *)
